11_017_998.lean
@@ -1,0 +1,213 @@
+import TuringMachine.Defs
+import TuringMachine.Lemmas
+import Mathlib.Tactic.Linarith.Frontend
+
+def transition : State5 -> Symbol2 -> Option State5 × Symbol2 × Direction
+  | State5.A, Symbol2.V0 => (some State5.B, Symbol2.V1, Direction.right)
+  | State5.A, Symbol2.V1 => (some State5.A, Symbol2.V1, Direction.left )
+  | State5.B, Symbol2.V0 => (some State5.C, Symbol2.V0, Direction.left )
+  | State5.B, Symbol2.V1 => (some State5.E, Symbol2.V0, Direction.right)
+  | State5.C, Symbol2.V0 => (none,          Symbol2.V1, Direction.right)
+  | State5.C, Symbol2.V1 => (some State5.D, Symbol2.V1, Direction.left )
+  | State5.D, Symbol2.V0 => (some State5.A, Symbol2.V1, Direction.right)
+  | State5.D, Symbol2.V1 => (some State5.C, Symbol2.V0, Direction.left )
+  | State5.E, Symbol2.V0 => (some State5.A, Symbol2.V1, Direction.right)
+  | State5.E, Symbol2.V1 => (some State5.E, Symbol2.V1, Direction.right)
+
+abbrev TM_11017998 := TuringMachine transition
+
+-- In state A and tape filled with zeroes 
+def starting_machine : TM_11017998 := 
+  TuringMachine.mk (Tape.blank Symbol2.V0) (State5.A)
+
+namespace proof
+
+-- state: B
+-- tape: n*[1] + [0] + (2n+1)*[1] + B0
+def B (n : Nat) : TuringMachine transition :=
+  let left_tape : Stream' Symbol2 := 
+    (2*n+1) ** [Symbol2.V1] ++
+                Symbol2.V0  ::
+       n    ** [Symbol2.V1] ++ₛ
+    Stream'.const Symbol2.V0
+  let tape : Tape Symbol2 := Tape.mk left_tape Symbol2.V0 (Stream'.const Symbol2.V0)
+  TuringMachine.mk tape State5.B
+
+-- state: C
+-- tape: (nm + nr) * [1] + [0] + nm * [11] + C1 + nr * [01]
+def B' (nm nr : Nat) : TM_11017998 :=
+  let left_tape : Stream' Symbol2 :=
+    (2*nm)  ** [Symbol2.V1] ++
+                Symbol2.V0  ::
+    (nm+nr) ** [Symbol2.V1] ++ₛ
+    Stream'.const Symbol2.V0
+  let right_tape : Stream' Symbol2 :=
+    nr  ** [Symbol2.V0, Symbol2.V1] ++ₛ
+    Stream'.const Symbol2.V0
+  TuringMachine.mk (Tape.mk left_tape Symbol2.V1 right_tape) State5.C
+
+-- state: A
+-- tape: nl * [1] + [0] + nml * [1] + A1 + nmr * [1] + nr * [01]
+def M (nl nml nmr nr : Nat) : TM_11017998 :=
+  let left_tape : Stream' Symbol2 :=
+    nml ** [Symbol2.V1] ++
+            Symbol2.V0  ::
+    nl  ** [Symbol2.V1] ++ₛ
+    Stream'.const Symbol2.V0
+  let right_tape : Stream' Symbol2 :=
+    nmr ** [Symbol2.V1]             ++
+    nr  ** [Symbol2.V0, Symbol2.V1] ++ₛ
+    Stream'.const Symbol2.V0
+  TuringMachine.mk (Tape.mk left_tape Symbol2.V1 right_tape) State5.A
+
+-- state: E
+-- tape: nl * [1] + [0] + nml * [1] + E1 + nmr * [1] + nr * [01]
+def M' (nl nml nmr nr : Nat) : TM_11017998 :=
+  let left_tape : Stream' Symbol2 :=
+    nml ** [Symbol2.V1] ++
+            Symbol2.V0  ::
+    nl  ** [Symbol2.V1] ++ₛ
+    Stream'.const Symbol2.V0
+  let right_tape : Stream' Symbol2 :=
+    nmr ** [Symbol2.V1]             ++
+    nr  ** [Symbol2.V0, Symbol2.V1] ++ₛ
+    Stream'.const Symbol2.V0
+  TuringMachine.mk (Tape.mk left_tape Symbol2.V1 right_tape) State5.E
+
+lemma reaches_B0 : starting_machine =>> B 0 := by
+  exists 1
+  ext : 1
+  . ext : 1
+    . have t2 : (B 0).tape.left_half = [Symbol2.V1] ++ₛ ([Symbol2.V0] ++ₛ Stream'.const Symbol2.V0) :=
+        by apply append_assoc
+      simp [t2, cons_to_const]
+      rfl
+    repeat rfl
+  . rfl
+
+lemma B_to_B'_ : B (nm + nr) =>> B' nm nr := by
+  cases nr with
+  | zero =>
+    exists 1
+    ext : 1
+    . ext : 1
+      repeat rfl
+      . have t1 : (TuringMachine.advance (B nm)).tape.right_half 
+          = [Symbol2.V0] ++ₛ (Stream'.const Symbol2.V0) := rfl
+        simp [t1, cons_to_const]
+        rfl
+    . rfl
+  | succ nr' =>
+    have t1 : nm + (nr' + 1) = (nm + 1) + nr' := by linarith
+    calc B (nm + (nr' + 1))
+      _ =   B ((nm + 1) + nr') := by rw [t1]
+      _ =>> B' (nm + 1) nr' := B_to_B'_ (nm := nm + 1) (nr := nr')
+      _ =>> B' nm (nr' + 1) := by
+        exists 2
+        unfold B'
+        ext : 2
+        simp [t1]
+        repeat rfl
+
+lemma B'_to_M_ (h : nml + nmr ≠ 0) : B' 0 (nml + nmr - 1) =>> M 0 nml nmr (nml + nmr - 1) := by
+  cases nmr with
+  | zero =>
+    exists 2
+    simp at h
+    have ⟨nml', hnml'⟩ := Nat.exists_eq_succ_of_ne_zero h
+    rw [hnml']
+    simp
+    ext : 1
+    . ext : 1
+      . unfold M; simp
+        have t1 : (TuringMachine.advance^[2] (B' 0 nml')).tape.left_half = 
+           Symbol2.V1 :: (0 + nml') ** [Symbol2.V1] ++ₛ Stream'.const Symbol2.V0 := rfl
+        simp [Nat.zero_add] at t1
+        have t2 : Symbol2.V0 :: 0 ** [Symbol2.V1] ++ₛ Stream'.const Symbol2.V0 = Stream'.const Symbol2.V0 := by
+          apply cons_to_const
+        rw [t1, append_assoc, t2]
+        rfl
+      . rfl
+      . unfold M
+        simp
+        rfl
+    . rfl
+  | succ nmr' =>
+    have t1 : nml + (nmr' + 1) = (nml + 1) + nmr' := by linarith
+    have t2 : (nml + 1) + nmr' ≠ 0 := by simp
+    calc B' 0 (nml + (nmr' + 1) - 1)
+      _ =   B' 0 ((nml + 1) + nmr' - 1) := by rw [t1]
+      _ =>> M 0 (nml + 1) nmr' ((nml + 1) + nmr' - 1) := B'_to_M_ t2
+      _ =   M 0 (nml + 1) nmr' (nml + nmr') := by simp
+      _ =>> M 0 nml (nmr' + 1) (nml + (nmr' + 1) - 1) := by exists 1
+
+lemma M_to_M'_ : M nl 0 (nml + nmr + 1) nr =>> M' (nl + 1) nml nmr nr := by
+  cases nml with
+  | zero => exists 3; simp; rfl
+  | succ nml' =>
+    have t1 : (nml' + 1) + nmr = nml' + (nmr + 1) := by linarith
+    calc M nl 0 ((nml' + 1) + nmr + 1) nr
+      _ =   M nl 0 (nml' + (nmr + 1) + 1) nr := by rw [t1]
+      _ =>> M' (nl + 1) nml' (nmr + 1) nr := M_to_M'_
+      _ =>> M' (nl + 1) (nml' + 1) nmr nr := by exists 1
+
+lemma M'_to_M_ : M' nl (nml + nmr) 0 (nr + 1) =>> M nl nml (nmr + 2) nr := by
+  cases nmr with
+  | zero => exists 4
+  | succ nmr' =>
+    have t1 : nml + (nmr' + 1) = (nml + 1) + nmr' := by linarith
+    calc M' nl (nml + (nmr' + 1)) 0 (nr + 1)
+      _ = M' nl ((nml + 1) + nmr') 0 (nr + 1) := by rw [t1]
+      _ =>> M nl (nml + 1) (nmr' + 2) nr := M'_to_M_
+      _ =>> M nl nml (nmr' + 3) nr := by exists 1
+
+lemma B_to_M' : B (nl + nr) =>> M' (nl + 1) (nr + 2 * nl) 0 nr := by
+  cases nl with
+  | zero =>
+    have t1 : 0 + (nr + 1) ≠ 0 := by simp
+    simp
+    calc B nr
+      _ = B (0 + nr) := by simp
+      _ =>> B' 0 nr := B_to_B'_
+      _ =   B' 0 (0 + (nr + 1) - 1) := by simp
+      _ =>> M 0 0 (nr + 1) (0 + (nr + 1) - 1) := B'_to_M_ (nml := 0) (nmr := nr + 1) t1
+      _ =   M 0 0 (nr + 1) nr := by simp
+      M 0 0 (nr + 0 + 1) nr =>> M' 1 nr 0 nr := M_to_M'_ (nl := 0) (nml := nr) (nmr := 0) (nr := nr)
+  | succ nl' =>
+    have t1 : (nl' + 1) + nr = nl' + (nr + 1) := by linarith
+    have t2 : nr + 1 + 2 * nl' + 2 = nr + 2 * (nl' + 1) + 0 + 1 := by linarith
+    calc B ((nl' + 1) + nr)
+      _ = B (nl' + (nr + 1)) := by rw [t1]
+      _ =>> M' (nl' + 1) (nr + 1 + 2 * nl') 0 (nr + 1) := B_to_M' (nl := nl') (nr := nr + 1)
+      _ =   M' (nl' + 1) (0 + (nr + 1 + 2 * nl')) 0 (nr + 1) := by simp
+      _ =>> M  (nl' + 1) 0 (_ + 2) nr := M'_to_M_ (nl := nl' + 1) (nr := nr) (nml := 0) (nmr := nr + 1 + 2 * nl')
+      _ =   M  (nl' + 1) 0 (nr + 2 * (nl' + 1) + 0 + 1) nr := by rw [t2]
+      _ =>> M' (nl' + 2) (nr + 2 * (nl' + 1)) 0 nr := M_to_M'_ (nml := nr + 2 * (nl' + 1)) (nmr := 0) (nr := nr)
+
+theorem B_to_B : B n =>> B (n + 1) := by
+  calc B n
+    _ =  B (n + 0) := by simp
+    _ =>> M' (n + 1) (0 + 2 * n) 0 0 := B_to_M'
+    _ =>> B (n + 1) := by simp; exists 3
+
+lemma B_ne_B : B n ≠ B (n + 1) := by
+  intro h
+  unfold B at h
+  simp at h
+  have h' := congr_arg (fun s => s (2 * n + 1)) h
+  simp at h'
+  rw [append_assoc, append_assoc] at h'
+  have t1 : 2 * n + 1 < 2 * (n + 1) + 1 := by linarith
+  conv at h' => rhs; rw [append_get' t1]
+  conv at h' => arg 1; arg 3; rw [←Nat.one_mul (2 * n + 1)]  
+  have t2 : List.length [Symbol2.V1] * (2 * n + 1) + 0 = 1 * (2 * n + 1) := by rfl
+  rw [←t2] at h'
+  rw [append_get (k := (2 * n + 1)) (l := [Symbol2.V1]) (n := 0) (s := (Symbol2.V0 :: n ** [Symbol2.V1] ++ₛ Stream'.const Symbol2.V0))] at h'
+  have t3 : Symbol2.V0 = Symbol2.V1 := h'
+  have t4 : Symbol2.V0 ≠ Symbol2.V1 := by decide
+  exact t4 t3
+
+theorem tm_not_halt : TuringMachine.does_not_halt starting_machine :=
+  tm_not_halt' B starting_machine @B_to_B @B_ne_B reaches_B0
+
+end proof
