7_763_480.lean
@@ -1,0 +1,116 @@
+import TuringMachine.Defs
+import TuringMachine.Lemmas
+import Mathlib.Tactic.Linarith.Frontend
+
+def transition : State5 -> Symbol2 -> Option State5 × Symbol2 × Direction
+  | State5.A, Symbol2.V0 => (some State5.B, Symbol2.V1, Direction.right)
+  | State5.A, Symbol2.V1 => (some State5.E, Symbol2.V0, Direction.left )
+  | State5.B, Symbol2.V0 => (some State5.C, Symbol2.V1, Direction.right)
+  | State5.B, Symbol2.V1 => (some State5.B, Symbol2.V1, Direction.right)
+  | State5.C, Symbol2.V0 => (some State5.D, Symbol2.V1, Direction.right)
+  | State5.C, Symbol2.V1 => (some State5.C, Symbol2.V1, Direction.left )
+  | State5.D, Symbol2.V0 => (some State5.E, Symbol2.V0, Direction.left )
+  | State5.D, Symbol2.V1 => (some State5.B, Symbol2.V0, Direction.right)
+  | State5.E, Symbol2.V0 => (none         , Symbol2.V1, Direction.right)
+  | State5.E, Symbol2.V1 => (some State5.A, Symbol2.V1, Direction.left )
+
+abbrev TM_7763480 := TuringMachine transition
+
+-- In state A and tape filled with zeroes
+def starting_machine : TM_7763480 :=
+  TuringMachine.mk (Tape.blank Symbol2.V0) (State5.A)
+
+namespace proof
+
+-- state: D
+-- tape: n*[1] + [0] + (2n+3)*[1] + D0
+def D (n : Nat) : TM_7763480 :=
+  let left_tape : Stream' Symbol2 :=
+    (2*n+3) ** [Symbol2.V1] ++
+                Symbol2.V0  ::
+       n    ** [Symbol2.V1] ++ₛ
+    Stream'.const Symbol2.V0
+  let tape : Tape Symbol2 := Tape.mk left_tape Symbol2.V0 (Stream'.const Symbol2.V0)
+  TuringMachine.mk tape State5.D
+
+-- state: E
+-- tape: (nm+nr) * [1] + [0] + nm * [11] + E1 + (nr+1)*[01]
+def D' (nm nr : Nat) : TM_7763480 :=
+  let left_tape : Stream' Symbol2 :=
+    (2*nm) ** [Symbol2.V1] ++
+    Symbol2.V0 ::
+    (nm + nr) ** [Symbol2.V1] ++ₛ
+    Stream'.const Symbol2.V0
+  let right_tape : Stream' Symbol2 :=
+    (nr + 1) ** [Symbol2.V0, Symbol2.V1] ++ₛ
+    Stream'.const Symbol2.V0
+  TuringMachine.mk (Tape.mk left_tape Symbol2.V1 right_tape) State5.E
+
+-- state: C
+-- tape: nl * [1] + [0] + nml * [1] + C1 + nmr * [1] + nr*[01]
+def C (nl nml nmr nr : Nat) : TM_7763480 :=
+  let left_tape : Stream' Symbol2 :=
+    nml ** [Symbol2.V1] ++
+    Symbol2.V0 ::
+    nl ** [Symbol2.V1] ++ₛ
+    Stream'.const Symbol2.V0
+  let right_tape : Stream' Symbol2 :=
+    nmr ** [Symbol2.V1] ++
+    nr ** [Symbol2.V0, Symbol2.V1] ++ₛ
+    Stream'.const Symbol2.V0
+  TuringMachine.mk (Tape.mk left_tape Symbol2.V1 right_tape) State5.E
+
+-- state: B
+-- tape: nl * [1] + [0] + nml * [1] + C1 + nmr * [1] + nr*[01]
+def C' (nl nml nmr nr : Nat) : TM_7763480 :=
+  let left_tape : Stream' Symbol2 :=
+    nml ** [Symbol2.V1] ++
+    Symbol2.V0 ::
+    nl ** [Symbol2.V1] ++ₛ
+    Stream'.const Symbol2.V0
+  let right_tape : Stream' Symbol2 :=
+    nmr ** [Symbol2.V1] ++
+    nr ** [Symbol2.V0, Symbol2.V1] ++ₛ
+    Stream'.const Symbol2.V0
+  TuringMachine.mk (Tape.mk left_tape Symbol2.V1 right_tape) State5.B
+
+lemma reaches_D0 : starting_machine =>> D 0 := by
+  exists 3
+  unfold D
+  simp [append_assoc, cons_to_const]
+  rfl
+
+lemma D_to_D' : D (nm + nr) =>> D' nm nr := by
+  cases nr with
+  | zero =>
+    exists 3
+    ext : 1
+    . ext : 1
+      repeat rfl
+      . have t1 : (TuringMachine.advance^[3] (D nm)).tape.right_half
+          = [Symbol2.V0, Symbol2.V1] ++ [Symbol2.V0] ++ₛ Stream'.const Symbol2.V0 := rfl
+        rw [Nat.add_zero, t1, append_assoc, cons_to_const]
+        rfl
+    . rfl
+  | succ nr' =>
+    have t1 : nm + (nr' + 1) = (nm + 1) + nr' := by linarith
+    calc D (nm + (nr' + 1))
+      _ =   D ((nm + 1) + nr') := by rw [t1]
+      _ =>> D' (nm + 1) nr' := D_to_D'
+      _ =>> D' nm (nr' + 1) := by
+        exists 2
+        ext : 1
+        . ext : 1
+          . unfold D'
+            rw [t1]
+            rfl
+          repeat rfl
+        . rfl
+
+lemma D'_to_C : D' 0 (nr + 1) =>> C 0 (nr + 3) 0 nr := by
+  admit
+
+theorem tm_not_halt : starting_machine.does_not_halt :=
+  sorry
+
+end proof
